src/3d/prelude/EverParse3d.Readable.fst
@@ -1,188 +1,79 @@
 module EverParse3d.Readable
 
-module B = LowStar.Buffer
-module HS = FStar.HyperStack
-module HST = FStar.HyperStack.ST
-module U32 = FStar.UInt32
-module G = FStar.Ghost
-module Seq = FStar.Seq
+let perm b = (p: B.pointer (Ghost.erased (Seq.lseq bool (B.length b))) {
+  B.loc_disjoint (B.loc_buffer b) (B.loc_buffer p)
+})
 
-module F = EverParse3d.Flags
+let loc_perm p = B.loc_buffer p
 
-inline_for_extraction
-noextract
-let perm' (#t: Type0) (b: B.buffer t)
-: Tot Type0
-= B.lbuffer (G.erased bool) (B.length b)
+let loc_perm_prop p = ()
 
-let perm #t b = if F.model then perm' b else unit
-  
-let loc_perm #t #b p = if F.model then B.loc_buffer (p <: perm' b) else B.loc_none
-
-let loc_perm_prop #t #b p = ()
-
-let valid_perm h #t #b p =
+let valid_perm h #_ #b p =
   B.live h b /\
-  B.loc_buffer b `B.loc_disjoint` loc_perm p /\
-  (F.model ==> B.live h (p <: perm' b))
+  B.live h p
 
-let valid_perm_prop h #t #b p = ()
+let valid_perm_prop h p = ()
 
-let valid_perm_frame h #t #b p l h' = ()
+let preserved #_ #b p from to h h' =
+  (valid_perm h p /\ U32.v from <= U32.v to /\ U32.v to <= B.length b) ==>
+  (valid_perm h' p /\ Seq.slice (B.deref h' p) (U32.v from) (U32.v to) `Seq.equal` Seq.slice (B.deref h p) (U32.v from) (U32.v to))
 
-let perm_gsub #t #b p offset length = if F.model then B.gsub (p <: perm' b) offset length else ()
+let valid_perm_frame h p l h' = ()
 
-let perm_sub #t #b p offset length = if F.model then B.sub (p <: perm' b) offset length else ()
+let preserved_refl p from to h = ()
 
-let perm_offset #t #b p offset = if F.model then B.offset (p <: perm' b) offset else ()
+let preserved_trans p from to h1 h2 h3 = ()
 
-let perm_gsub_gsub #t #b p offset1 length1 offset2 length2 = ()
+let preserved_split p from mid to h h' =
+  let s = B.deref h p in
+  let s' = B.deref h' p in
+  assert (Seq.slice s' (U32.v from) (U32.v to) `Seq.equal` (Seq.slice s' (U32.v from) (U32.v mid) `Seq.append` Seq.slice s' (U32.v mid) (U32.v to)));
+  assert (Seq.slice s (U32.v from) (U32.v to) `Seq.equal` (Seq.slice s (U32.v from) (U32.v mid) `Seq.append` Seq.slice s (U32.v mid) (U32.v to)));
+  assert (Seq.slice s' (U32.v from) (U32.v mid) `Seq.equal` Seq.slice (Seq.slice s' (U32.v from) (U32.v to)) 0 (U32.v mid - U32.v from));
+  assert (Seq.slice s' (U32.v mid) (U32.v to) `Seq.equal` Seq.slice (Seq.slice s' (U32.v from) (U32.v to)) (U32.v mid - U32.v from) (U32.v to - U32.v from))
 
-let perm_gsub_zero_length #t #b p =
-  B.gsub_zero_length b;
-  if F.model then B.gsub_zero_length (p <: perm' b)
-
-let loc_perm_gsub #t #b p offset length = ()
-
-let valid_perm_gsub h #t #b p offset length = ()
-
-let loc_perm_from_to_disjoint #t #b p from1 to1 from2 to2 = ()
-
-let readable h #t #b p from to =
+let readable h p from to =
   valid_perm h p /\
-  (F.model ==> B.as_seq h (B.gsub p from (to `U32.sub` from)) `Seq.equal` Seq.create (U32.v to - U32.v from) (G.hide true))
+  Seq.slice (B.deref h p) (U32.v from) (U32.v to) `Seq.equal` Seq.create (U32.v to - U32.v from) true
 
-let readable_prop h #t #b p from to = ()
+let readable_prop h p from to = ()
 
-let readable_gsub h #t #b p offset length from to = ()
+let readable_split h p from mid to =
+  let s = B.deref h p in
+  assert (Seq.slice s (U32.v from) (U32.v to) `Seq.equal` (Seq.slice s (U32.v from) (U32.v mid) `Seq.append` Seq.slice s (U32.v mid) (U32.v to)));
+  assert (Seq.slice s (U32.v from) (U32.v mid) `Seq.equal` Seq.slice (Seq.slice s (U32.v from) (U32.v to)) 0 (U32.v mid - U32.v from));
+  assert (Seq.slice s (U32.v mid) (U32.v to) `Seq.equal` Seq.slice (Seq.slice s (U32.v from) (U32.v to)) (U32.v mid - U32.v from) (U32.v to - U32.v from));
+  assert (Seq.create (U32.v to - U32.v from) true `Seq.equal` (Seq.create (U32.v mid - U32.v from) true `Seq.append` Seq.create (U32.v to - U32.v mid) true))
 
-let readable_split_1
-  (h: HS.mem)
-  (#t: _) (#b: B.buffer t) (p: perm b)
-  (from: U32.t)
-  (mid: U32.t)
-  (to: U32.t { U32.v from <= U32.v mid /\ U32.v mid <= U32.v to /\ U32.v to <= B.length b })
-: Lemma
-  (requires (readable h p from to))
-  (ensures (readable h p from mid /\ readable h p mid to))
-= if F.model then begin
-    let s_from_to = B.as_seq h (B.gsub (p <: perm' b) from (to `U32.sub` from)) in
-    let s_from_mid = B.as_seq h (B.gsub (p <: perm' b) from (mid `U32.sub` from)) in
-    let s_mid_to = B.as_seq h (B.gsub (p <: perm' b) mid (to `U32.sub` mid)) in
+let readable_frame0 h p from to h' = ()
 
-    assert (forall (i:nat). i < Seq.length s_from_to ==> Seq.index s_from_to i == G.hide true);
+let unreadable h p from to =
+  valid_perm h p ==>
+  (Seq.slice (B.deref h p) (U32.v from) (U32.v to) `Seq.equal` Seq.create (U32.v to - U32.v from) false)
 
-    assert (forall (i:nat). i < Seq.length s_from_mid ==> Seq.index s_from_mid i == G.hide true);
-    assert (readable h p from mid);
+let unreadable_prop h p from to = ()
 
-    assert (forall (i:nat). i < Seq.length s_mid_to ==> Seq.index s_mid_to i == Seq.index s_from_to (i+ U32.v mid-U32.v from));
-    assert (forall (i:nat). i < Seq.length s_mid_to ==> Seq.index s_mid_to i == G.hide true);
-    assert (readable h p mid to)
-  end
+let readable_not_unreadable h p from to =
+  assert (~ (Seq.index (Seq.create (U32.v to - U32.v from) true) 0 == Seq.index (Seq.create (U32.v to - U32.v from) false) 0))
 
-#push-options "--fuel 17 --z3rlimit 32" // "--using_facts_from '*,-LowParse.Low.Base.serializer32_of_leaf_writer_strong_constant_size'"
-#restart-solver
+let unreadable_split h p from mid to =
+  let s = B.deref h p in
+  assert (Seq.slice s (U32.v from) (U32.v to) `Seq.equal` (Seq.slice s (U32.v from) (U32.v mid) `Seq.append` Seq.slice s (U32.v mid) (U32.v to)));
+  assert (Seq.slice s (U32.v from) (U32.v mid) `Seq.equal` Seq.slice (Seq.slice s (U32.v from) (U32.v to)) 0 (U32.v mid - U32.v from));
+  assert (Seq.slice s (U32.v mid) (U32.v to) `Seq.equal` Seq.slice (Seq.slice s (U32.v from) (U32.v to)) (U32.v mid - U32.v from) (U32.v to - U32.v from));
+  assert (Seq.create (U32.v to - U32.v from) false `Seq.equal` (Seq.create (U32.v mid - U32.v from) false `Seq.append` Seq.create (U32.v to - U32.v mid) false))
 
-let readable_split_2
-  (h: HS.mem)
-  (#t: _) (#b: B.buffer t) (p: perm b)
-  (from: U32.t)
-  (mid: U32.t)
-  (to: U32.t { U32.v from <= U32.v mid /\ U32.v mid <= U32.v to /\ U32.v to <= B.length b })
-: Lemma
-  (requires (readable h p from mid /\ readable h p mid to))
-  (ensures (readable h p from to))
-=
-  Seq.lemma_split (B.as_seq h (B.gsub b from (to `U32.sub` from))) (U32.v mid - U32.v from);
-  if F.model then Seq.lemma_split (B.as_seq h (B.gsub (p <: perm' b) from (to `U32.sub` from))) (U32.v mid - U32.v from)
+let unreadable_empty h p i = ()
 
-#pop-options
-#restart-solver
+let unreadable_frame0 h p from to h' = ()
 
-let readable_split h #t #b p from mid to =
-  Classical.move_requires (readable_split_1 h p from mid) to;
-  Classical.move_requires (readable_split_2 h p from mid) to
+let unreadable_frame h p from to l h' = ()
 
-let readable_frame h #t #b p from to l h' = ()
-
-let unreadable h #t #b p from to =
-  (valid_perm h p /\ F.model) ==>
-  B.as_seq h (B.gsub p from (to `U32.sub` from)) `Seq.equal` Seq.create (U32.v to - U32.v from) (G.hide false)
-
-let unreadable_prop h #t #b p from to = ()
-
-let model = FStar.Ghost.hide F.model
-
-let readable_not_unreadable h #t #b p from to =
-  let f () : Lemma
-    (requires (F.model /\ readable h p from to /\ unreadable h p from to))
-    (ensures False)
-  = assert (valid_perm h p);
-    let s = B.as_seq h (B.gsub p from (to `U32.sub` from)) in
-    assert (s == Seq.create (U32.v to - U32.v from) (G.hide true));
-    assert (Seq.index s 0 == G.hide true);
-    assert (s == Seq.create (U32.v to - U32.v from) (G.hide false));
-    assert (Seq.index s 0 == G.hide false);
-    assert False
-  in
-  Classical.move_requires f ()
-
-let unreadable_gsub h #t #b p offset length from to = ()
-
-#push-options "--warn_error -271"
-let unreadable_split_1
-  (h: HS.mem)
-  (#t: _) (#b: B.buffer t) (p: perm b)
-  (from: U32.t)
-  (mid: U32.t)
-  (to: U32.t { U32.v from <= U32.v mid /\ U32.v mid <= U32.v to /\ U32.v to <= B.length b })
-: Lemma
-  (requires (unreadable h p from to))
-  (ensures (unreadable h p from mid /\ unreadable h p mid to))
-=
-  let aux (#a:Type) (s:Seq.seq a) (from to mid:nat) (x:a)
-    : Lemma
-        (requires
-          from <= mid /\ mid <= to /\ to <= Seq.length s /\
-          Seq.equal (Seq.slice s from to) (Seq.create (to - from) x))
-        (ensures Seq.equal (Seq.slice s from mid)
-                           (Seq.create (mid - from) x) /\
-                 Seq.equal (Seq.slice s mid to)
-                           (Seq.create (to - mid) x))
-        [SMTPat ()]
-    = 
-    let aux0 (#a:Type) (s:Seq.seq a) (from:nat) (to:nat{from <= to /\ to <= Seq.length s})
-        (i:nat{from <= i /\ i < to})
-        : Lemma (Seq.index (Seq.slice s from to) (i - from) == Seq.index s i)
-                [SMTPat ()]
-        = Seq.lemma_index_slice s from to (i - from) in
-      assert (forall (i:nat). (from <= i /\ i < to) ==> Seq.index (Seq.slice s from to) (i - from) == x);
-      assert (forall (i:nat). (from <= i /\ i < to) ==> Seq.index s i == x) in
-  ()
-#pop-options
-
-#push-options "--z3rlimit 16"
-#restart-solver
-let unreadable_split_2
-  (h: HS.mem)
-  (#t: _) (#b: B.buffer t) (p: perm b)
-  (from: U32.t)
-  (mid: U32.t)
-  (to: U32.t { U32.v from <= U32.v mid /\ U32.v mid <= U32.v to /\ U32.v to <= B.length b })
-: Lemma
-  (requires (unreadable h p from mid /\ unreadable h p mid to))
-  (ensures (unreadable h p from to))
-= Seq.lemma_split (B.as_seq h (B.gsub b from (to `U32.sub` from))) (U32.v mid - U32.v from);
-  if F.model then Seq.lemma_split (B.as_seq h (B.gsub (p <: perm' b) from (to `U32.sub` from))) (U32.v mid - U32.v from)
-#pop-options
-
-let unreadable_split h #t #b p from mid to =
-  Classical.move_requires (unreadable_split_1 h p from mid) to;
-  Classical.move_requires (unreadable_split_2 h p from mid) to
-
-let unreadable_empty h #t #b p i = ()
-
-let unreadable_frame h #t #b p from to l h' = ()
-
-let drop #t #b p from to =
-  if F.model then B.fill (B.sub (p <: perm' b) from (to `U32.sub` from)) (G.hide false) (to `U32.sub` from) else ()
+let drop p from to =
+  let open LowStar.BufferOps in
+  let r = !* p in
+  p *= Ghost.hide (
+    Seq.slice r 0 (U32.v from) `Seq.append`
+    Seq.create (U32.v to - U32.v from) false `Seq.append`
+    Seq.slice r (U32.v to) (Seq.length r)
+  )
